MS+SI for Hacl.AES_128_GCM.M32

code/experimental/aes-gcm/Hacl.AES_128_GCM.M32.fst
@@ -11,7 +11,7 @@ open Hacl.Gf128.PreComp
 module ST = FStar.HyperStack.ST
 
 
-#set-options "--z3rlimit 500"
+#reset-options "--z3rlimit 1500 --max_fuel 1"
 
 let aes_gcm_ctx_len = 396ul
 
@@ -82,6 +82,8 @@ let aes128_gcm_encrypt ctx len out text aad_len aad =
   pop_frame()
 
 
+#reset-options "--z3rlimit 1500 --max_fuel 1"
+
 val aes128_gcm_decrypt:
     ctx: aes_gcm_ctx
   -> len: size_t{v len + 16 <= max_size_t}
@@ -96,41 +98,47 @@ val aes128_gcm_decrypt:
                  /\ disjoint ctx aad
                  /\ disjoint out cipher
                  /\ disjoint out aad))
-  (ensures (fun h0 r h1 -> modifies1 out h0 h1))
-
-#reset-options "--z3rlimit 500 --max_fuel 1"
+  (ensures (fun h0 r h1 -> modifies2 out ctx h0 h1))
 
 let aes128_gcm_decrypt ctx len out cipher aad_len aad =
   push_frame();
-  let scratch = create 16ul (u8 0) in
+  let scratch = create 18ul (u8 0) in
+  let text = sub scratch 0ul 16ul in
+  let zero = sub scratch 16ul 1ul in
+  let result = sub scratch 17ul 1ul in
   let ciphertext = sub cipher 0ul len in
+  let tag = sub cipher len (size 16) in
   let aes_ctx = sub ctx (size 0) (size 128) in
   let gcm_ctx = sub ctx (size 128) (size 266) in
   let tag_mix = sub ctx (size 394) (size 2) in
+  let h1 = ST.get () in
   gcm_update_blocks_padded gcm_ctx aad_len aad;
   gcm_update_blocks_padded gcm_ctx len ciphertext;
   uint_to_bytes_be #U64 (sub scratch (size 0) (size 8)) (to_u64 (aad_len *. size 8));
   uint_to_bytes_be #U64 (sub scratch (size 8) (size 8)) (to_u64 (len *. size 8));
-  gcm_update_blocks gcm_ctx (size 16) scratch;
-  gcm_emit scratch gcm_ctx;
+  gcm_update_blocks gcm_ctx (size 16) text;
+  gcm_emit text gcm_ctx;
   let scratch0 = uint_from_bytes_le #U64 (sub scratch 0ul 8ul) in
   let scratch1 = uint_from_bytes_le #U64 (sub scratch 8ul 8ul) in
   let scratch0 = scratch0 ^. tag_mix.(0ul) in
   let scratch1 = scratch1 ^. tag_mix.(1ul) in
   uint_to_bytes_le #U64 (sub scratch 0ul 8ul) scratch0;
   uint_to_bytes_le #U64 (sub scratch 8ul 8ul) scratch1;
-  let tag = sub cipher len (size 16) in
-  let res = create 1ul (u8 0) in
-  let h1 = ST.get() in
-  loop_nospec #h1 (size 16) res
-    (fun i -> res.(0ul) <- res.(0ul) |. (scratch.(i) ^. tag.(i)));
-  let r = res.(size 0) in
-  admit();
-  if Lib.RawIntTypes.u8_to_UInt8 r = 0uy then (
-    let cip = sub cipher (size 0) len in
-    aes128_ctr len out cip aes_ctx (size 2);
-    pop_frame();
-    true)
-  else (
-    pop_frame();
-    false)
+  let h7 = ST.get () in
+  loop_nospec #h7 (size 16) result
+    (fun i -> result.(0ul) <- result.(0ul) |. (scratch.(i) ^. tag.(i)));
+  let h8 = ST.get () in
+  assert(modifies2 ctx scratch h1 h8);
+  let res8 = result.(0ul) in
+  let r =
+    if Lib.RawIntTypes.u8_to_UInt8 res8 = 0uy then (
+      aes128_ctr len out ciphertext aes_ctx (size 2);
+      true)
+    else (
+      let h9 = ST.get () in
+      modifies2_is_modifies3 ctx scratch out h1 h9;
+      assert(modifies3 out ctx scratch h1 h9);
+      false)
+  in
+  pop_frame();
+  r
